src/Quarantine.fst
@@ -1,6 +1,9 @@
 module Quarantine
 
-let quarantine_slab arr = if enable_quarantine_trap then trap_array arr else A.varray arr
+let quarantine_slab arr =
+  if enable_quarantine_trap
+  then trap_array arr
+  else A.varray arr
 
 let mmap_trap_quarantine arr len =
   if enable_quarantine_trap then (
@@ -13,4 +16,13 @@ let mmap_trap_quarantine arr len =
   ) else (
     noop ();
     change_equal_slprop (A.varray arr) (quarantine_slab arr)
+  )
+
+let mmap_untrap_quarantine arr len =
+  if enable_quarantine_trap then (
+    change_equal_slprop (quarantine_slab arr) (trap_array arr);
+    mmap_untrap arr len
+  ) else (
+    noop ();
+    change_equal_slprop (quarantine_slab arr) (A.varray arr)
   )
