src/MemoryTrap.fsti
@@ -44,3 +44,13 @@ val mmap_trap
   : SteelT unit
   (A.varray arr)
   (fun _ -> trap_array arr)
+
+/// Elimination function for the abstract `trap_array`
+/// predicate above. Under the hood, this function will
+/// be implemented in C as a mmap(PROT_READ|PROT_WRITE)
+val mmap_untrap
+  (arr: array U8.t)
+  (len: US.t{US.v len == A.length arr /\ US.v len > 0})
+  : SteelT unit
+  (trap_array arr)
+  (fun _ -> A.varray arr)
